Wavelet/Compile.lean
@@ -1,3 +1,4 @@
 import Wavelet.Compile.Fn
 import Wavelet.Compile.Prog
+import Wavelet.Compile.MapChans
 import Wavelet.Compile.AffineOp
