Wavelet/Compile/MapChans.lean
@@ -1,0 +1,51 @@
+import Wavelet.Dataflow.Proc
+
+/-! Renaming channels of a `Proc`/`AtomicProc` -/
+
+namespace Wavelet.Dataflow
+
+open Semantics
+
+def AtomicProc.mapChans [Arity Op] (f : χ → χ') : AtomicProc Op χ V → AtomicProc Op χ' V
+  | .op o inputs outputs => .op o (inputs.map f) (outputs.map f)
+  | .switch decider inputs outputs₁ outputs₂ =>
+    .switch (f decider) (inputs.map f) (outputs₁.map f) (outputs₂.map f)
+  | .steer flavor decider inputs outputs =>
+    .steer flavor (f decider) (inputs.map f) (outputs.map f)
+  | .carry inLoop decider inputs₁ inputs₂ outputs =>
+    .carry inLoop (f decider) (inputs₁.map f) (inputs₂.map f) (outputs.map f)
+  | .merge decider inputs₁ inputs₂ outputs =>
+    .merge (f decider) (inputs₁.map f) (inputs₂.map f) (outputs.map f)
+  | .forward inputs outputs => .forward (inputs.map f) (outputs.map f)
+  | .fork input outputs => .fork (f input) (outputs.map f)
+  | .const c act outputs => .const c (f act) (outputs.map f)
+  | .forwardc inputs consts outputs => .forwardc (inputs.map f) consts (outputs.map f)
+  | .sink inputs => .sink (inputs.map f)
+
+def AtomicProcs.mapChans [Arity Op] (f : χ → χ')
+  : AtomicProcs Op χ V → AtomicProcs Op χ' V
+  := List.map (AtomicProc.mapChans f)
+
+def Proc.mapChans [Arity Op] (f : χ → χ') (p : Proc Op χ V m n) : Proc Op χ' V m n :=
+  {
+    inputs := p.inputs.map f,
+    outputs := p.outputs.map f,
+    atoms := p.atoms.mapChans f,
+  }
+
+section Simulation
+
+theorem sim_map_chans_inj
+  {χ χ' : Type u}
+  [Arity Op]
+  [DecidableEq χ]
+  [DecidableEq χ']
+  [InterpConsts V]
+  {f : χ → χ'}
+  {proc : Proc Op χ V m n}
+  (hf : Function.Injective f) :
+  proc.semantics ≲ (proc.mapChans f).semantics := sorry
+
+end Simulation
+
+end Wavelet.Dataflow
